Examples/arm7_collatz_smc_proof.v
@@ -12,35 +12,37 @@ Definition collatz_start : N :=  0x100.
 Definition collatz_end   : N :=  0x100 + 4 * 7.
 
 Section Invariants.
-  Variables inp : N.
+  Variable  base: addr.
+  Variable  inp : N.
   Variable  s0 : store.
 
   Definition postcondition (s:store) :=
     s R_R0 = if N.even inp then inp >> 1 else inp ⊕ (1 ⊕ inp >> 1).
   Definition mem_unchanged (s:store) := s V_MEM32 = s0 V_MEM32.
   Definition invs (t:trace) : option Prop:=
-    match t with (Addr a, s) :: _ => match a with
-      | 0x100 => Some (mem_unchanged s /\ s R_R0 = inp /\ s R_T = 0 /\ s R_JF = 0 /\ s R_E = 0)
-      | 0x11c => Some (postcondition s)
-      | _ => None end
+    match t with (Addr a, s) :: _ =>
+    if a =? base then
+      Some (mem_unchanged s /\ s R_R0 = inp /\ s R_T = 0 /\ s R_JF = 0 /\ s R_E = 0)
+    else if a =? base + 0x1c then
+      Some (postcondition s)
+    else None
     | _ => None end.
 End Invariants.
 
-Definition collatz_exit (t:trace) :=
-  match t with (Addr a,_)::_ => match a with
-  | 0x11c => true
-  | _ => false
-  end | _ => false end.
+Definition collatz_exit (base:addr) (t:trace) :=
+  match t with (Addr a,_)::_ => a =? base+0x1c | _ => false end.
 
 Theorem collatz_correctness:
-  forall s t s' x' inp
-         (ENTRY: startof t (x',s') = (Addr 0x100,s))
+  forall s t s' x' inp base
+         (ENTRY: startof t (x',s') = (Addr base,s))
          (MDL: models arm7typctx s)
          (RT: s R_T = 0)
          (JF: s R_JF = 0)
          (RE: s R_E = 0)
          (INP: s R_R0 = inp)
-         (MEM: collatz_arm7 s)
+         (BASE: base < 2^32 - 32)
+         (BASEM: base mod 4 = 0)
+         (MEM: collatz_arm7 base s)
 ,
 (* We define our program as p32_prog, a function that looks into
    a given store's memory and page-execute permissions to determine
@@ -48,7 +50,7 @@ Theorem collatz_correctness:
    Above we specified that the memory of the initial store is exactly
    our program, which is held in bytes 0-12 with all other bytes 0.
 *)
-  satisfies_all arm_prog (invs inp s) collatz_exit ((x',s')::t).
+  satisfies_all arm_prog (invs base inp s) (collatz_exit base) ((x',s')::t).
 Proof.
 Local Ltac step := time ISA_step.
 intros. unfold satisfies_all.
@@ -67,18 +69,25 @@ intros. unfold satisfies_all.
   erewrite startof_prefix in ENTRY; try eassumption.
   eapply models_at_invariant; try (eassumption || apply welltyped_arm_prog).
   clear MDL; intros MDL.
-  clear - PRE MDL MEM. rename s into s0, t1 into t, s1 into s.
+  clear - PRE MDL MEM BASE BASEM. rename s into s0, t1 into t, s1 into s.
 
-  destruct_inv 32 PRE.
+  destruct (N.eq_dec a1 base); try subst a1.
+  2: {
+    unfold get_precondition, collatz_exit, invs in PRE.
+    destruct (a1 =? base + 28). contradiction.
+    rewrite <-N.eqb_neq in n; rewrite n in PRE. contradiction.
+  }
+
+  prep_precondition PRE.
   destruct PRE as (MEMSAME & INP & RT & JF & RE).
   unfold collatz_arm7 in MEM.
   rewrite <-MEMSAME in *. clear MEMSAME.
   step.
   step.
   step.
-  step.
-  step.
-  step.
+  step. (* Takes 38s on my machine. Why? *)
+  step. (* Takes 50s on my machine. Why? *)
+  step. (* Takes 50s on my machine... *)
 
   assert (inp mod 2 < 2) by lia.
   destruct (inp mod 2) as [|p] eqn:EQ; try destruct p; try lia.
@@ -101,7 +110,6 @@ intros. unfold satisfies_all.
   specialize (H1 1 inp 1). psimpl in H1. assert (HELP: n+1>=1) by lia.
   specialize (H1 EQ (eq_refl _) (n+1) HELP); clear HELP.
   rewrite H1.
-  Unset Printing Notations.
   admit.
 
   step.
